WIP: fix collatz

dataplane/Examples/Collatz.thy
@@ -10,6 +10,7 @@ imports
   Tmap_op
   Concat_op
   Branch_op
+  Increment_op
 begin
 
 abbreviation init_input_state where
@@ -20,9 +21,9 @@ abbreviation init_input_state where
    produ = [],
    input = (\<lambda> _. []),
    outpu = (\<lambda> _. []),
-   front = Code.abort (STR ''Frontier of op1 not initialized'') (\<lambda> _ _. antichain_from_list []),
+   front = Code.abort (STR ''Frontier not initialized'') (\<lambda> _ _. antichain_from_list []),
    ocaps = (\<lambda> _. [\<bottom>]),
-   initia = False,
+   initia = True,
    nfron = False,
    en1 = id,
    de1 = id,
@@ -37,9 +38,9 @@ abbreviation init_operator_state where
    produ = [],
    input = (\<lambda> _. []),
    outpu = (\<lambda> _. []),
-   front = Code.abort (STR ''Frontier of op2 not initialized'') (\<lambda> _ _. antichain_from_list []),
+   front = Code.abort (STR ''Frontier not initialized'') (\<lambda> _ _. antichain_from_list []),
    ocaps = (\<lambda> _. []),
-   initia = False,
+   initia = True,
    nfron = False
    \<rparr>"
 
@@ -51,9 +52,9 @@ abbreviation init_operator_state_ty2 where
    produ = [],
    input = (\<lambda> _. []),
    outpu = (\<lambda> _. []),
-   front = Code.abort (STR ''Frontier of op2 not initialized'') (\<lambda> _ _. antichain_from_list []),
+   front = Code.abort (STR ''Frontier not initialized'') (\<lambda> _ _. antichain_from_list []),
    ocaps = (\<lambda> _. []),
-   initia = False,
+   initia = True,
    nfron = False,
    en1 = id,
    de1 = id,
@@ -61,12 +62,13 @@ abbreviation init_operator_state_ty2 where
    de2 = id
    \<rparr>"
 
-abbreviation "nid0 \<equiv> (0 :: 4)"
-abbreviation "nid1 \<equiv> (1 :: 4)"
-abbreviation "nid2 \<equiv> (2 :: 4)"
-abbreviation "nid3 \<equiv> (2 :: 4)"
-abbreviation "p0 \<equiv> (0 :: 2)"
-abbreviation "p1 \<equiv> (1 :: 2)"
+definition "nid0 = 0"
+definition "nid1 = 1"
+definition "nid2 = 2"
+definition "nid3 = 3"
+definition "nid4 = (4 :: 5)"
+definition "p0 = (0 :: 2)"
+definition "p1 = (1 :: 2)"
 
 abbreviation "logic_map nid op \<equiv> map_op (case_option (Inl nid) (\<lambda> p. Inr (nid, p))) (case_option (Inl nid) (\<lambda> p. Inr (nid, p))) op"
 
@@ -77,31 +79,50 @@ abbreviation "coll_op nid \<equiv> logic_map nid (collatz_op init_operator_state
 
 abbreviation "conc_op nid \<equiv> logic_map nid (concat_op {|p0, p1|} p0 init_operator_state)"
 
-abbreviation "bran_op nid \<equiv> logic_map nid (branch_op p0 p0 p1 (\<lambda> (x, t). t < 100) init_operator_state)"
+abbreviation "bran_op nid \<equiv> logic_map nid (branch_op p0 p0 p1 (\<lambda> (x, t). snd x \<le> 1 \<or> t > 100) init_operator_state)"
+
+abbreviation "incr_op nid \<equiv> logic_map nid (increment_op p1 p1 1 init_operator_state)"
 
 abbreviation "comp_op_map \<equiv> map_op (case_sum id id) (case_sum id id)"
 
 abbreviation "g0 \<equiv>
-   comp_op_map (comp_op [Inr (nid3, p0) \<mapsto> Inr (nid1, p0)] (\<lambda> _. []) (conc_op nid3) (coll_op nid1))"
+   comp_op_map (comp_op [Inr (nid0, p0) \<mapsto> Inr (nid1, p0)] (\<lambda> _. []) (conc_op nid0) (coll_op nid1))"
 
-abbreviation "g1 inps \<equiv>
-   comp_op_map (comp_op [Inr (nid0, p0) \<mapsto> Inr (nid1, p0)] (\<lambda> _. []) (inp_op nid0 inps) g0)"
+abbreviation "g1 \<equiv>
+   comp_op_map (comp_op [Inr (nid1, p0) \<mapsto> Inr (nid2, p0)] (\<lambda> _. []) g0 (bran_op nid2))"
 
-abbreviation "g2 inps \<equiv>
-   comp_op_map (comp_op [Inr (nid1, p0) \<mapsto> Inr (nid2, p0)] (\<lambda> _. []) (g1 inps) (bran_op nid2))"
+abbreviation "g2 \<equiv>
+   comp_op_map (comp_op [Inr (nid2, p1) \<mapsto> Inr (nid3, p1)] (\<lambda> _. []) g1 (incr_op nid3))"
 
+abbreviation "g3 \<equiv>
+   loop_op [Inr (nid3, p1) \<mapsto> Inr (nid0, p1)] (\<lambda> _. []) g2"
 
-abbreviation "inpp_op inps \<equiv>
-   ((inp_op nid0 inps))"
+abbreviation "g4 inps \<equiv>
+   comp_op_map (comp_op [Inr (nid4, p0) \<mapsto> Inr (nid0, p0)] (\<lambda> _. []) (inp_op nid4 inps) g3)"
 
-abbreviation "op \<equiv> g2 (\<lambda> p. llist_of [Data (0 :: nat) (5 :: nat, 5 :: nat)])"
+abbreviation "inps0 \<equiv> (\<lambda> p. llist_of []) :: 'a \<Rightarrow> (nat, nat \<times> nat) event llist"
+abbreviation "inps1 \<equiv> \<lambda> p. llist_of [Data (0 :: nat) (5 :: nat, 5 :: nat)]"
+
+abbreviation "op \<equiv> g4 inps1"
 
 definition "my_summ = (\<lambda> l1 l2.
-   if l1 = Loc 0 (Src 1) \<and> l2 = Loc 1 (Trg 0) 
+   if l1 = Loc nid4 (Src p0) \<and> l2 = Loc nid0 (Trg p0) 
    then antichain_from_list [0]
-   else if l1 = Loc 0 (Trg 0) \<and> l2 = Loc 0 (Src 0)
+   else if l1 = Loc nid0 (Trg p0) \<and> l2 = Loc nid0 (Src p0)
    then antichain_from_list [0]
-   else if l1 = Loc 1 (Trg 0) \<and> l2 = Loc 1 (Src 0)
+   else if l1 = Loc nid0 (Src p0) \<and> l2 = Loc nid1 (Trg p0)
+   then antichain_from_list [0]
+   else if l1 = Loc nid1 (Trg p0) \<and> l2 = Loc nid1 (Src p0)
+   then antichain_from_list [0]
+   else if l1 = Loc nid1 (Src p0) \<and> l2 = Loc nid2 (Trg p0)
+   then antichain_from_list [0]
+   else if l1 = Loc nid2 (Trg p0) \<and> l2 = Loc nid2 (Src p0)
+   then antichain_from_list [0]
+   else if l1 = Loc nid2 (Src p1) \<and> l2 = Loc nid3 (Trg p1)
+   then antichain_from_list [0]
+   else if l1 = Loc nid3 (Trg p1) \<and> l2 = Loc nid3 (Src p1)
+   then antichain_from_list [1]
+   else if l1 = Loc nid3 (Src p1) \<and> l2 = Loc nid0 (Trg p1)
    then antichain_from_list [0]
    else {}\<^sub>A)"
 
@@ -117,15 +138,13 @@ value [GHC] r
 
 value [GHC] "p0"
 value [GHC] "p1"
+(* 
+value [GHC] "check_prefix 30 [((nid2, p0), ((1, 1), 0))] dt"
 
-value [GHC] nid0
-value [GHC] nid1
-value [GHC] nid2
-
-(* export_code r in Haskell module_name Test2
  *)
 (* 
-value [GHC] "check_prefix [VOut (1, 1) ((2, 2), 0)] dt"
+ export_code r in Haskell module_name Test6
  *)
+
 
 end
