dataplane/Examples/Branch_op.thy
@@ -6,7 +6,7 @@ begin
 
 definition \<open>branch_op ip p0 p1 c os = builder_op False {|ip|} {|p0, p1|} os (\<lambda> os. {|
       let result = input os ip in
-      let os = produces os (map (\<lambda> (d, t). (d, Cap t (if c d then trace (STR ''p0!'') p0 else trace (STR ''p1!'') p1))) result) in
+      let os = produces os (map (\<lambda> (d, t). (d, Cap t (if c (d, t) then trace (STR ''p0!'') p0 else trace (STR ''p1!'') p1))) result) in
       let os = drop_caps os (map (\<lambda> t. Cap t p0) (ocaps os p0) @ map (\<lambda> t. Cap t p1) (ocaps os p1) ) in
       os\<lparr> input := (\<lambda> p. []) \<rparr>
     |}
