dataplane/Examples/Concat_op.thy
@@ -5,9 +5,10 @@ imports
 begin
 
 definition \<open>concat_op ips p os = builder_op False ips {|p|} os (\<lambda> os. {|
-      let result = concat (map (\<lambda> p. input os p) Enum.enum) in
-      let os = produces os (map (\<lambda> (d, t). (d, Cap t 1)) result) in
-      let os = drop_caps os (map (\<lambda> t. Cap t 1) (ocaps os 1)) in
+      let result = concat (map (\<lambda> p. input os p) [x <- Enum.enum. x |\<in>| ips]) in
+      let os = produces os (map (\<lambda> (d, t). (d, Cap t p)) result) in
+      let os = drop_caps os (concat (map (\<lambda> p. map (\<lambda> t. Cap t p) (ocaps os p)) Enum.enum)) in
+      trace (STR ''concat_op!'')
       os\<lparr> input := (\<lambda> p. []) \<rparr>
     |}
    )\<close>
